Definition for memory partialization
In the same way that stacks are partialized by applying a dedicated
partialization function that hides the details of its implementation, we
add the missing function that performs the analogous process for
memories. This makes code more readable and will be of use to write
lemmas on partialized memories. With the proofs as they currently stand,
the introduction of the change involves some unfolding of the definition
at appropriate points, but no further changes are needed.

A further abstraction may be possible by having these partializer
functions operate on a piece of the state (stack, memory) and, instead
of the domain of a program interface, on the program interface itself.

Intermediate/PS.v
@@ -174,13 +174,19 @@ Proof.
       rewrite (IHgps1 gps2); auto.
 Qed.
 
+(* Memory partialization, *)
+
+(* RB: TODO: Here and above, Program.interface vs. fset. *)
+Definition to_partial_memory (mem : Memory.t) (ctx : {fset Component.id}) :=
+  filterm (fun k _ => negb (k \in ctx)) mem.
+
 Inductive partial_state (ctx: Program.interface) : CS.state -> PS.state -> Prop :=
 | ProgramControl: forall gps pgps mem pmem regs pc,
     (* program has control *)
     is_program_component (PC (pgps, pmem, regs, pc)) ctx ->
 
     (* we forget about context memories *)
-    pmem = filterm (fun k _ => negb (k \in domm ctx)) mem ->
+    pmem = to_partial_memory mem (domm ctx) ->
 
     (* we put holes in place of context information in the stack *)
     pgps = to_partial_stack gps (domm ctx) ->
@@ -192,7 +198,7 @@ Inductive partial_state (ctx: Program.interface) : CS.state -> PS.state -> Prop 
     is_context_component (CC (Pointer.component pc, pgps, pmem)) ctx ->
 
     (* we forget about context memories *)
-    pmem = filterm (fun k _ => negb (k \in domm ctx)) mem ->
+    pmem = to_partial_memory mem (domm ctx) ->
 
     (* we put holes in place of context information in the stack *)
     pgps = to_partial_stack gps (domm ctx) ->
@@ -204,10 +210,10 @@ Definition partialize (ics: CS.state) (ctx: Program.interface) : PS.state :=
   if Pointer.component pc \in domm ctx then
     CC (Pointer.component pc,
         to_partial_stack gps (domm ctx),
-        filterm (fun k _ => negb (k \in domm ctx)) mem)
+        to_partial_memory mem (domm ctx))
   else
     PC (to_partial_stack gps (domm ctx),
-        filterm (fun k _ => negb (k \in domm ctx)) mem,
+        to_partial_memory mem (domm ctx),
         regs, pc).
 
 Lemma partialize_correct:
@@ -326,7 +332,7 @@ Proof.
   rewrite mem_domm. simpl.
   rewrite domm0.
   rewrite unpartializing_complete_stack.
-  rewrite filterm_identity. reflexivity.
+  unfold to_partial_memory. rewrite filterm_identity. reflexivity.
 Qed.
 
 (* merging partial states *)
@@ -865,14 +871,14 @@ Proof.
       try (symmetry; assumption).
     + rewrite Pointer.inc_preserves_component.
       destruct ptr as [[]].
-      erewrite context_store_in_partialized_memory; eauto.
+      unfold to_partial_memory. erewrite context_store_in_partialized_memory; eauto.
       * rewrite Pointer.inc_preserves_component.
         rewrite <- H18. eassumption.
     + erewrite find_label_in_component_1 with (pc:=pc); eauto.
     + rewrite H18. reflexivity.
     + erewrite find_label_in_procedure_1 with (pc:=pc); eauto.
     + rewrite Pointer.inc_preserves_component.
-      erewrite context_allocation_in_partialized_memory; eauto.
+      unfold to_partial_memory. erewrite context_allocation_in_partialized_memory; eauto.
       * rewrite Pointer.inc_preserves_component.
         eassumption.
 Qed.
@@ -1120,6 +1126,8 @@ Proof.
     inversion Hpartial2'
       as [cstk2' ? cmem2' ? regs2' pc2' Hpc2' | cstk2' ? cmem2' ? regs2' pc2' Hcc2'];
       subst;
+    (* (Now that we are done inverting, expose this definition.) *)
+    unfold to_partial_memory in *;
     try discharge_pc_cc Hcomp Hcc1';
     try discharge_pc_cc Hcomp Hcc2';
     (* For the remaining goals, unify components of their matching opcodes and their
